fairneris/partial_termination.v
@@ -1,0 +1,307 @@
+From Paco Require Import pacotac.
+From stdpp Require Import finite.
+From iris.proofmode Require Import proofmode.
+From trillium Require Import adequacy.
+From fairneris Require Import fairness retransmit_model_progress_ltl.
+From fairneris.aneris_lang Require Import aneris_lang resources.
+From fairneris.aneris_lang.state_interp Require Import state_interp_def.
+From fairneris.aneris_lang.state_interp Require Import state_interp_config_wp.
+From fairneris.aneris_lang.state_interp Require Import state_interp.
+From fairneris.aneris_lang.program_logic Require Import aneris_weakestpre.
+From fairneris Require Import from_locale_utils trace_utils ltl_lite.
+
+
+Definition snd_proj {A1 A2 B1 B2} (l : (A1 * A2) + (B1 * B2)) : (A2 + B2) :=
+  sum_map snd snd l.
+
+Definition ex_send_filter msg : cfg aneris_lang → option $ ex_label aneris_lang → Prop :=
+  λ _ l, option_map (sum_map snd id) l = Some $ inl $ Some msg.
+Instance ex_send_filter_decision msg st l : Decision (ex_send_filter msg st l).
+Proof. apply make_decision. Qed.
+
+
+Definition ex_deliver_filter msg : cfg aneris_lang → option $ ex_label aneris_lang → Prop :=
+  λ _ l, option_map (sum_map snd id) l = Some $ inr $ Some msg.
+Instance ex_deliver_filter_decision msg st l : Decision (ex_deliver_filter msg st l).
+Proof. apply make_decision. Qed.
+
+(* Definition retransmit_fair_network_delivery msg : mtrace → Prop := *)
+(*   □ (□◊↓send_filter msg → ◊↓deliver_filter msg). *)
+Definition retransmit_fair_network_delivery_ex msg : extrace aneris_lang → Prop :=
+  □ (□◊↓ex_send_filter msg → ◊↓ex_deliver_filter msg).
+
+Definition retransmit_fair_network_ex (extr : extrace aneris_lang) : Prop :=
+  ∀ msg, retransmit_fair_network_delivery_ex msg extr.
+
+(* TODO: Clean up this definition (annoying to state lemmas about,
+         due to separate labels) *)
+Definition live_tid (c : cfg aneris_lang) (δ : retransmit_state)
+  (ℓ:retransmit_node_role) (ζ:locale aneris_lang) : Prop :=
+  roles_match ζ ℓ →
+  role_enabled_model (ℓ:fmrole retransmit_fair_model) δ ↔ locale_enabled ζ c.
+
+Definition live_tids (c : cfg aneris_lang) (δ : retransmit_state) : Prop :=
+  ∀ ℓ ζ, live_tid c δ ℓ ζ.
+
+Definition live_traces_match : extrace aneris_lang → mtrace → Prop :=
+  traces_match labels_match live_tids language.locale_step retransmit_trans.
+
+Lemma traces_match_valid_preserved extr mtr :
+  live_traces_match extr mtr → mtrace_valid mtr.
+Proof. Admitted.
+
+Definition extrace_fair (extr : extrace aneris_lang) :=
+  (∀ ζ, fair_scheduling_ex ζ extr) ∧ retransmit_fair_network_ex extr.
+
+Lemma traces_match_cons_inv {S1 S2 L1 L2}
+      (Rℓ: L1 -> L2 -> Prop) (Rs: S1 -> S2 -> Prop)
+      (trans1: S1 -> L1 -> S1 -> Prop)
+      (trans2: S2 -> L2 -> S2 -> Prop)
+      s1 s2 l1 l2 tr1 tr2 :
+  traces_match Rℓ Rs trans1 trans2 (s1 -[l1]-> tr1) (s2 -[l2]-> tr2) ->
+  Rs s1 s2 ∧ Rℓ l1 l2.
+Proof. intros Hm. inversion Hm; done. Qed.
+
+Lemma labels_match_deliver_filter_impl msg s1 s2 ℓ1 ℓ2 extr mtr :
+  labels_match ℓ1 ℓ2 →
+  (↓ ex_deliver_filter msg) (s1 -[ ℓ1 ]-> extr) →
+  (↓ deliver_filter msg) (s2 -[ ℓ2 ]-> mtr).
+Proof.
+  intros Hmatch Hmtr.
+  rewrite /trace_now /pred_at /ex_deliver_filter in Hmtr.
+  rewrite /trace_now /pred_at /deliver_filter. simpl in *.
+  destruct ℓ1; simplify_eq.
+  destruct ℓ2; [done|].
+  rewrite /labels_match /locale_retransmit_label in Hmatch.
+  by simplify_eq.
+Qed.
+
+Lemma labels_match_send_filter_impl msg s1 s2 ℓ1 ℓ2 extr mtr :
+  labels_match ℓ1 ℓ2 →
+  (↓ send_filter msg) (s2 -[ ℓ2 ]-> mtr) →
+  (↓ ex_send_filter msg) (s1 -[ ℓ1 ]-> extr).
+Proof.
+  intros Hmatch Hmtr.
+  rewrite /trace_now /pred_at /send_filter in Hmtr.
+  rewrite /trace_now /pred_at /ex_send_filter. simpl in *.
+  simplify_eq.
+  destruct ℓ2; simplify_eq.
+  assert (r.2 = Some msg) as Heq1.
+  { destruct r.
+    rewrite /label_action /locale_retransmit_label in Hmtr.
+    simpl in *. by simplify_eq. }
+  destruct ℓ1; simplify_eq; last first.
+  { rewrite /labels_match /locale_retransmit_label in Hmatch.
+    simplify_eq. }
+  assert (l.2 = r.2) as Heq2.
+  { rewrite /labels_match /locale_retransmit_label in Hmatch.
+    destruct l.
+    destruct (locale_retransmit_role l); [|done].
+    simpl in *. simplify_eq. simpl. done. }
+  simpl. rewrite Heq2 Heq1. done.
+Qed.
+
+Lemma fair_network_impl extr mtr :
+  live_traces_match extr mtr →
+  retransmit_fair_network_ex extr → retransmit_fair_network mtr.
+Proof.
+  rewrite /retransmit_fair_network_ex /retransmit_fair_network.
+  intros Hmatch Hfairex_network.
+  assert (mtrace_valid mtr) as Hvalid.
+  { by eapply traces_match_valid_preserved. }
+  intros msg.
+  specialize (Hfairex_network msg).
+  rewrite /retransmit_fair_network_delivery_ex in Hfairex_network.
+  rewrite trace_alwaysI in Hfairex_network.
+  rewrite /retransmit_fair_network_delivery.
+  rewrite trace_alwaysI.
+  intros mtr' [n Hmtr'].
+  pose proof Hmtr' as Hextr'.
+  eapply traces_match_after in Hextr'; [|done].
+  destruct Hextr' as (extr'&Hextr'&Hmatch').
+  specialize (Hfairex_network extr').
+  assert (trace_suffix_of extr' extr) as Hsuffix.
+  { eexists _. done. }
+  apply Hfairex_network in Hsuffix.
+  rewrite trace_impliesI.
+  rewrite trace_impliesI in Hsuffix.
+  intros Hmtr''.
+  assert ((□ ◊ ↓ ex_send_filter msg) extr') as Hextr''.
+  { rewrite trace_alwaysI.
+    intros extr'' [m Hextr''].
+    eapply traces_match_flip in Hmatch'.
+    pose proof Hextr'' as Hmtr'''.
+    eapply traces_match_after in Hmtr'''; [|done].
+    destruct Hmtr''' as (mtr''&Hmtr'''&Hmatch'').
+    rewrite trace_alwaysI in Hmtr''.
+    specialize (Hmtr'' mtr'').
+    assert (trace_suffix_of mtr'' mtr') as Hsuffix'.
+    { eexists _. done. }
+    apply Hmtr'' in Hsuffix'.
+    rewrite trace_eventuallyI in Hsuffix'.
+    destruct Hsuffix' as [mtr''' [Hsuffix' Hmtr'''']].
+    destruct Hsuffix' as [m'' Hsuffix'].
+    apply traces_match_flip in Hmatch''.
+    eapply traces_match_after in Hmatch''; [|done].
+    destruct Hmatch'' as [extr''' [Hextr''' Hmatch''']].
+    destruct mtr'''; [done|].
+    simpl in *.
+    rewrite trace_eventuallyI. exists extr'''.
+    split; [eexists _;done|].
+    destruct extr'''; [by inversion Hmatch'''|].
+    assert (labels_match ℓ0 ℓ) as Hlabels.
+    { by eapply traces_match_cons_inv. }
+    by eapply labels_match_send_filter_impl. }
+  apply Hsuffix in Hextr''.
+  rewrite trace_eventuallyI in Hextr''.
+  destruct Hextr'' as [extr'' [[m Hsuffix''] Hextr'']].
+  rewrite trace_eventuallyI.
+  eapply traces_match_flip in Hmatch'.
+  eapply traces_match_after in Hmatch'; [|done].
+  destruct Hmatch' as [mtr'' [Hmtr''' Hmatch'']].
+  exists mtr''. split; [by eexists _|].
+  destruct extr''; [done|].
+  destruct mtr''; [by inversion Hmatch''|].
+  assert (labels_match ℓ ℓ0) as Hlabels.
+  { eapply traces_match_cons_inv. apply traces_match_flip. done. }
+  by eapply labels_match_deliver_filter_impl.
+Qed.
+
+Definition retransmit_role_locale (ρ : retransmit_node_role) : locale aneris_lang :=
+  match ρ with
+  | Arole => ("0.0.0.0",0)
+  | Brole => ("0.0.0.1",0)
+  end.
+
+Lemma locale_retransmit_role_cancel ρ :
+  locale_retransmit_role (retransmit_role_locale ρ) = Some ρ.
+Proof. by destruct ρ. Qed.
+
+Lemma fair_scheduling_impl extr mtr :
+  live_traces_match extr mtr →
+  (∀ ζ, fair_scheduling_ex ζ extr) → retransmit_fair_scheduling mtr.
+Proof.
+  rewrite /fair_scheduling_ex /retransmit_fair_scheduling.
+  intros Hmatch Hextr ρ.
+  rewrite /retransmit_fair_scheduling_mtr.
+  rewrite /trace_always_eventually_implies_now.
+  rewrite /trace_always_eventually_implies.
+  rewrite trace_alwaysI.
+  intros mtr' [n Hmtr_after]. rewrite trace_impliesI.
+  intros Hρ.
+  eapply traces_match_after in Hmatch; [|done].
+  destruct Hmatch as [extr' [Hextr_after Hmatch]].
+  specialize (Hextr (retransmit_role_locale ρ) n).
+  rewrite /pred_at in Hextr.
+  rewrite Hextr_after in Hextr.
+  assert (match extr' with
+          | ⟨ s ⟩ | s -[ _ ]-> _ => locale_enabled (retransmit_role_locale ρ) s
+          end) as Hextr'.
+  { apply traces_match_first in Hmatch.
+    destruct extr'.
+    - eapply (Hmatch ρ).
+      + destruct ρ; done.
+      + rewrite /trace_now /pred_at in Hρ. simpl in *.
+        by destruct mtr'.
+    - eapply (Hmatch ρ).
+      + destruct ρ; done.
+      + rewrite /trace_now /pred_at in Hρ. simpl in *.
+        by destruct mtr'. }
+  apply Hextr in Hextr' as [m Hextr'].
+  rewrite after_sum' Hextr_after in Hextr'.
+  destruct (after m extr') as [extr''|] eqn:Hextr_after'; last first.
+  { rewrite Hextr_after' in Hextr'. done. }
+  rewrite Hextr_after' in Hextr'.
+  rewrite trace_eventuallyI.
+  apply traces_match_flip in Hmatch.
+  eapply traces_match_after in Hmatch; [|done].
+  destruct Hmatch as [mtr'' [Hmtr_after' Hmatch]].
+  exists mtr''. split; [by eexists _|].
+  rewrite /trace_now /pred_at=> /=.
+  destruct mtr''.
+  - destruct extr''; [|by inversion Hmatch].
+    destruct Hextr' as [Hextr'|Hextr']; [|done].
+    left. intros Hs. apply Hextr'.
+    apply traces_match_first in Hmatch.
+    eapply (Hmatch ρ).
+    + destruct ρ; done.
+    + rewrite /trace_now /pred_at in Hρ. simpl in *. done.
+  - destruct extr''; [by inversion Hmatch|].
+    destruct Hextr' as [Hextr'|Hextr'].
+    { left. intros Hs. apply Hextr'.
+      apply traces_match_first in Hmatch.
+      eapply (Hmatch ρ).
+      + destruct ρ; done.
+      + rewrite /trace_now /pred_at in Hρ. simpl in *. done. }
+    right. simpl in *. simplify_eq.
+    apply traces_match_cons_inv in Hmatch as [_ Hmatch].
+    rewrite /labels_match in Hmatch.
+    destruct ℓ0; [|done].
+    simpl in *. destruct l. simpl in *. simplify_eq.
+    rewrite locale_retransmit_role_cancel in Hmatch.
+    simpl in *. simplify_eq.
+    done.
+Qed.
+
+Lemma traces_match_fairness_preserved extr mtr :
+  live_traces_match extr mtr →
+  extrace_fair extr → mtrace_fair mtr.
+Proof.
+  intros Hmatch [Hfairex_sched Hfairex_network].
+  split; [by eapply fair_scheduling_impl|by eapply fair_network_impl].
+Qed.
+
+Definition extrace_terminating_locale (ζ : locale aneris_lang) (tr : extrace aneris_lang) : Prop :=
+  (◊↓λ st _, ¬ locale_enabled ζ st) tr ∨ ¬ infinite_trace tr.
+
+Lemma terminating_role_preserved ρ ζ mtr extr :
+  live_traces_match extr mtr →
+  roles_match ζ ρ →
+  retransmit_terminating_role ρ mtr →
+  extrace_terminating_locale ζ extr.
+Proof.
+  intros Hmatch Hroles [Hρ|Hinf]; last first.
+  { right.
+    intros Hinf'. apply Hinf.
+    intros n. destruct (Hinf' n) as [extr' Hextr_after].
+    apply traces_match_flip in Hmatch.
+    eapply traces_match_after in Hmatch; [|done].
+    destruct Hmatch as [mtr' [Hmtr_after Hmatch]].
+    exists mtr'. done. }
+  left.
+  rewrite trace_eventuallyI in Hρ.
+  destruct Hρ as [mtr' [[n Hmtr_after] Hρ]].
+  rewrite trace_eventuallyI.
+  eapply traces_match_after in Hmatch; [|done].
+  destruct Hmatch as [extr' [Hextr_after Hmatch]].
+  exists extr'.
+  split; [by eexists _|].
+  rewrite /trace_now /pred_at.
+  rewrite /trace_now /pred_at in Hρ.
+  simpl in *.
+  destruct mtr'.
+  - destruct extr'; [|by inversion Hmatch].
+    apply traces_match_first in Hmatch.
+    intros Henabled.
+    apply Hρ.
+    clear Hρ.
+    by eapply Hmatch.
+  - destruct extr'; [by inversion Hmatch|].
+    apply traces_match_first in Hmatch.
+    intros Henabled.
+    apply Hρ.
+    clear Hρ.
+    by eapply Hmatch.
+Qed.
+
+Lemma fair_extrace_terminate extr mtr :
+  live_traces_match extr mtr →
+  extrace_valid extr → extrace_fair extr →
+  extrace_terminating_locale localeB extr.
+Proof.
+  intros Hmatch Hvalid Hfair.
+  eapply terminating_role_preserved; [done|done|].
+  apply retransmit_fair_traces_terminate;
+    [by eapply traces_match_valid_preserved|].
+  by eapply traces_match_fairness_preserved.
+Qed.
